cont (finished MP-Trie theory)

Experiments/Maximal_Path_Trie.thy
@@ -1,8 +1,14 @@
-theory IO_Tree
+theory Maximal_Path_Trie
 imports FSM
 begin
 
-subsection \<open>Utils\<close>
+section \<open>Maximal Path Tries\<close>
+
+text \<open>Drastically reduced implementation of tries that consider only maximum length sequences as elements.
+      Inserting a sequence that is prefix of some already contained sequence does not alter the trie.
+      Intended to store IO-sequences to apply in testing, as in this use-case proper prefixes need not be applied separately\<close>
+
+subsection \<open>Utils for Updating Associative Lists\<close>
 
 fun update_assoc_list_with_default :: "'a \<Rightarrow> ('b \<Rightarrow> 'b) \<Rightarrow> 'b \<Rightarrow> ('a \<times> 'b) list \<Rightarrow> ('a \<times> 'b) list" where
   "update_assoc_list_with_default k f d [] = [(k,f d)]" |
@@ -84,36 +90,36 @@ qed
 
 
 
-subsection \<open>IO Tries\<close>
+subsection \<open>Maximum Path Trie Implementation\<close>
 
 
-datatype 'a io_trie = IO_Trie "('a \<times> 'a io_trie) list"
+datatype 'a mp_trie = MP_Trie "('a \<times> 'a mp_trie) list"
 
-fun io_trie_invar :: "'a io_trie \<Rightarrow> bool" where
-  "io_trie_invar (IO_Trie ts) = (distinct (map fst ts) \<and> (\<forall> t \<in> set (map snd ts) . io_trie_invar t))"
-
-
-
-definition empty :: "'a io_trie" where
-  "empty = IO_Trie []"
-
-lemma empty_invar : "io_trie_invar empty" unfolding empty_def by auto
+fun mp_trie_invar :: "'a mp_trie \<Rightarrow> bool" where
+  "mp_trie_invar (MP_Trie ts) = (distinct (map fst ts) \<and> (\<forall> t \<in> set (map snd ts) . mp_trie_invar t))"
 
 
 
-fun height :: "'a io_trie \<Rightarrow> nat" where
-  "height (IO_Trie []) = 0" |
-  "height (IO_Trie (xt#xts)) = Suc (foldr (\<lambda> t m . max (height t) m) (map snd (xt#xts)) 0)"
+definition empty :: "'a mp_trie" where
+  "empty = MP_Trie []"
+
+lemma empty_invar : "mp_trie_invar empty" unfolding empty_def by auto
+
+
+
+fun height :: "'a mp_trie \<Rightarrow> nat" where
+  "height (MP_Trie []) = 0" |
+  "height (MP_Trie (xt#xts)) = Suc (foldr (\<lambda> t m . max (height t) m) (map snd (xt#xts)) 0)"
 
 lemma height_0 : 
   assumes "height t = 0" 
   shows "t = empty" 
 proof (rule ccontr)
   assume "t \<noteq> empty"
-  then obtain xt xts where "t = IO_Trie (xt#xts)"
-    by (metis IO_Tree.empty_def height.cases)
+  then obtain xt xts where "t = MP_Trie (xt#xts)"
+    by (metis empty_def height.cases)
   have "height t > 0" 
-    unfolding \<open>t = IO_Trie (xt#xts)\<close> height.simps
+    unfolding \<open>t = MP_Trie (xt#xts)\<close> height.simps
     by simp
   then show "False"
     using assms by simp
@@ -127,7 +133,7 @@ lemma max_by_foldr :
 
 lemma height_inc :
   assumes "t \<in> set (map snd ts)"
-  shows "height t < height (IO_Trie ts)"
+  shows "height t < height (MP_Trie ts)"
 proof -
   obtain xt xts where "ts = xt#xts"
     using assms
@@ -140,34 +146,24 @@ proof -
   then show ?thesis unfolding \<open>ts = xt#xts\<close> by auto
 qed
 
-(*
-lemma io_tree_induct :
-  assumes "P empty"
-  and     "\<And> ts . (\<And> t . t \<in> set (map snd ts) \<Longrightarrow> P t) \<Longrightarrow> P (IO_Trie ts)"
-shows "P t"
-*)
 
-
-
-
-
-fun insert :: "'a list \<Rightarrow> 'a io_trie \<Rightarrow> 'a io_trie" where
+fun insert :: "'a list \<Rightarrow> 'a mp_trie \<Rightarrow> 'a mp_trie" where
   "insert [] t = t" |
-  "insert (x#xs) (IO_Trie ts) = (IO_Trie (update_assoc_list_with_default x (\<lambda> t . insert xs t) empty ts))"
+  "insert (x#xs) (MP_Trie ts) = (MP_Trie (update_assoc_list_with_default x (\<lambda> t . insert xs t) empty ts))"
 
 
-lemma insert_invar : "io_trie_invar t \<Longrightarrow> io_trie_invar (insert xs t)" 
+lemma insert_invar : "mp_trie_invar t \<Longrightarrow> mp_trie_invar (insert xs t)" 
 proof (induction xs arbitrary: t)
   case Nil
   then show ?case by auto
 next
   case (Cons x xs)
 
-  obtain ts where "t = IO_Trie ts"
-    using io_trie_invar.cases by auto
+  obtain ts where "t = MP_Trie ts"
+    using mp_trie_invar.cases by auto
 
   then have "distinct (map fst ts)"
-       and  "\<And> t . t \<in> set (map snd ts) \<Longrightarrow> io_trie_invar t"
+       and  "\<And> t . t \<in> set (map snd ts) \<Longrightarrow> mp_trie_invar t"
     using Cons.prems by auto
     
   
@@ -175,27 +171,27 @@ next
     case True
     then obtain i where "i < length ts" and "fst (ts ! i) = x"
       by (metis in_set_conv_nth length_map nth_map) 
-    have "insert (x#xs) (IO_Trie ts) = (IO_Trie (take i ts @ [(x, insert xs (snd (ts ! i)))] @ drop (Suc i) ts))"
+    have "insert (x#xs) (MP_Trie ts) = (MP_Trie (take i ts @ [(x, insert xs (snd (ts ! i)))] @ drop (Suc i) ts))"
       unfolding insert.simps empty_def
-      unfolding update_assoc_list_with_default_key_found[OF \<open>distinct (map fst ts)\<close> \<open>i < length ts\<close> \<open>fst (ts ! i) = x\<close>, of "(\<lambda> t . insert xs t)" "(IO_Trie [])"] 
+      unfolding update_assoc_list_with_default_key_found[OF \<open>distinct (map fst ts)\<close> \<open>i < length ts\<close> \<open>fst (ts ! i) = x\<close>, of "(\<lambda> t . insert xs t)" "(MP_Trie [])"] 
       by simp
     
-    have "\<And> t . t \<in> set (map snd (take i ts @ [(x, insert xs (snd (ts ! i)))] @ drop (Suc i) ts)) \<Longrightarrow> io_trie_invar t"
+    have "\<And> t . t \<in> set (map snd (take i ts @ [(x, insert xs (snd (ts ! i)))] @ drop (Suc i) ts)) \<Longrightarrow> mp_trie_invar t"
     proof - 
       fix t assume "t \<in> set (map snd (take i ts @ [(x, insert xs (snd (ts ! i)))] @ drop (Suc i) ts))"
       then consider (a) "t \<in> set (map snd (take i ts @ drop (Suc i) ts))" |
                     (b) "t = insert xs (snd (ts ! i))" 
         by auto
-      then show "io_trie_invar t" proof cases
+      then show "mp_trie_invar t" proof cases
         case a
         then have "t \<in> set (map snd ts)"
           by (metis drop_map in_set_dropD in_set_takeD list_concat_non_elem map_append take_map) 
-        then show ?thesis using \<open>\<And> t . t \<in> set (map snd ts) \<Longrightarrow> io_trie_invar t\<close> by blast
+        then show ?thesis using \<open>\<And> t . t \<in> set (map snd ts) \<Longrightarrow> mp_trie_invar t\<close> by blast
       next
         case b
         have "(snd (ts ! i)) \<in> set (map snd ts)"
           using \<open>i < length ts\<close> by auto
-        then have "io_trie_invar (snd (ts ! i))" using \<open>\<And> t . t \<in> set (map snd ts) \<Longrightarrow> io_trie_invar t\<close> by blast 
+        then have "mp_trie_invar (snd (ts ! i))" using \<open>\<And> t . t \<in> set (map snd ts) \<Longrightarrow> mp_trie_invar t\<close> by blast 
         then show ?thesis using Cons.IH unfolding b by blast
       qed 
     qed
@@ -204,17 +200,17 @@ next
       by (metis \<open>distinct (map fst ts)\<close> \<open>fst (ts ! i) = x\<close> \<open>i < length ts\<close> update_assoc_list_with_default_key_found)
     
     ultimately show ?thesis 
-      unfolding \<open>t = IO_Trie ts\<close> \<open>insert (x#xs) (IO_Trie ts) = (IO_Trie (take i ts @ [(x, insert xs (snd (ts ! i)))] @ drop (Suc i) ts))\<close>
+      unfolding \<open>t = MP_Trie ts\<close> \<open>insert (x#xs) (MP_Trie ts) = (MP_Trie (take i ts @ [(x, insert xs (snd (ts ! i)))] @ drop (Suc i) ts))\<close>
       by auto
   next
     case False
 
-    have "io_trie_invar (IO_Tree.insert xs empty)"
+    have "mp_trie_invar (insert xs empty)"
       by (simp add: empty_invar Cons.IH) 
 
     then show ?thesis
-      using Cons.prems update_assoc_list_with_default_key_distinct[OF \<open>distinct (map fst ts)\<close>, of x "(IO_Tree.insert xs)" "(IO_Trie [])"]
-      unfolding \<open>t = IO_Trie ts\<close> insert.simps
+      using Cons.prems update_assoc_list_with_default_key_distinct[OF \<open>distinct (map fst ts)\<close>, of x "(insert xs)" "(MP_Trie [])"]
+      unfolding \<open>t = MP_Trie ts\<close> insert.simps
       unfolding update_assoc_list_with_default_key_not_found[OF \<open>distinct (map fst ts)\<close> False] 
       by auto
   qed
@@ -223,16 +219,16 @@ qed
 
 
 
-fun paths :: "'a io_trie \<Rightarrow> 'a list list" where
-  "paths (IO_Trie []) = [[]]" |
-  "paths (IO_Trie (t#ts)) = concat (map (\<lambda> (x,t) . map ((#) x) (paths t)) (t#ts))"
+fun paths :: "'a mp_trie \<Rightarrow> 'a list list" where
+  "paths (MP_Trie []) = [[]]" |
+  "paths (MP_Trie (t#ts)) = concat (map (\<lambda> (x,t) . map ((#) x) (paths t)) (t#ts))"
 
 
 
-value "insert [1,2,3,4] (empty :: nat io_trie)"
-value "insert [1,2,5,6] (insert [1,2,3,4] (empty :: nat io_trie))"
-value "insert [1,2,5,7] (insert [1,2,5,6] (insert [1,2,3,4] (empty :: nat io_trie)))"
-value "paths (insert [1,2,5,7] (insert [1,2,5,6] (insert [1,2,3,4] (empty :: nat io_trie))))"
+value "insert [1,2,3,4] (empty :: nat mp_trie)"
+value "insert [1,2,5,6] (insert [1,2,3,4] (empty :: nat mp_trie))"
+value "insert [1,2,5,7] (insert [1,2,5,6] (insert [1,2,3,4] (empty :: nat mp_trie)))"
+value "paths (insert [1,2,5,7] (insert [1,2,5,6] (insert [1,2,3,4] (empty :: nat mp_trie))))"
 
 
 
@@ -241,8 +237,8 @@ lemma paths_empty :
   shows "t = empty"
 proof (rule ccontr)
   assume "t \<noteq> empty"
-  then obtain xt xts where "t = IO_Trie (xt#xts)"
-    by (metis IO_Tree.empty_def height.cases)
+  then obtain xt xts where "t = MP_Trie (xt#xts)"
+    by (metis empty_def height.cases)
   then have "[] \<in> set (concat (map (\<lambda> (x,t) . map ((#) x) (paths t)) (xt#xts)))"
     using assms by auto
   then show "False" by auto
@@ -251,7 +247,7 @@ qed
 lemma paths_nonempty :
   assumes "[] \<notin> set (paths t)"
   shows "set (paths t) \<noteq> {}"
-using assms proof (induction t rule: io_trie_invar.induct)
+using assms proof (induction t rule: mp_trie_invar.induct)
   case (1 ts)
   have "ts \<noteq> []" using "1.prems" by auto
   then obtain x t xts where "ts = ((x,t)#xts)"
@@ -274,7 +270,7 @@ using assms proof (induction t rule: io_trie_invar.induct)
 qed
 
 
-lemma paths_maximal: "io_trie_invar t \<Longrightarrow> xs' \<in> set (paths t) \<Longrightarrow> \<not> (\<exists> xs'' . xs'' \<noteq> [] \<and> xs'@xs'' \<in> set (paths t))"
+lemma paths_maximal: "mp_trie_invar t \<Longrightarrow> xs' \<in> set (paths t) \<Longrightarrow> \<not> (\<exists> xs'' . xs'' \<noteq> [] \<and> xs'@xs'' \<in> set (paths t))"
 proof (induction xs' arbitrary: t)
   case Nil
   then have "t = empty"
@@ -286,40 +282,40 @@ next
   case (Cons x xs')
 
   then have "t \<noteq> empty" unfolding empty_def by auto
-  then obtain xt xts where "t = IO_Trie (xt#xts)"
-    by (metis IO_Tree.empty_def height.cases)
+  then obtain xt xts where "t = MP_Trie (xt#xts)"
+    by (metis empty_def height.cases)
 
   obtain t' where "(x,t') \<in> set (xt#xts)"
             and   "xs' \<in> set (paths t')"
     using Cons.prems(2) 
-    unfolding \<open>t = IO_Trie (xt#xts)\<close> paths.simps 
+    unfolding \<open>t = MP_Trie (xt#xts)\<close> paths.simps 
     by force
 
-  have "io_trie_invar t'"
-    using Cons.prems(1) \<open>(x,t') \<in> set (xt#xts)\<close> unfolding \<open>t = IO_Trie (xt#xts)\<close> by auto
+  have "mp_trie_invar t'"
+    using Cons.prems(1) \<open>(x,t') \<in> set (xt#xts)\<close> unfolding \<open>t = MP_Trie (xt#xts)\<close> by auto
 
   show ?case 
   proof 
     assume "\<exists>xs''. xs'' \<noteq> [] \<and> (x # xs') @ xs'' \<in> set (paths t)"
-    then obtain xs'' where "xs'' \<noteq> []" and "(x # (xs' @ xs'')) \<in> set (paths (IO_Trie (xt # xts)))"
-      unfolding \<open>t = IO_Trie (xt#xts)\<close> by force
+    then obtain xs'' where "xs'' \<noteq> []" and "(x # (xs' @ xs'')) \<in> set (paths (MP_Trie (xt # xts)))"
+      unfolding \<open>t = MP_Trie (xt#xts)\<close> by force
 
 
     obtain t'' where "(x,t'') \<in> set (xt#xts)"
                and   "(xs' @ xs'') \<in> set (paths t'')"
-      using \<open>(x # (xs' @ xs'')) \<in> set (paths (IO_Trie (xt # xts)))\<close>
-      unfolding \<open>t = IO_Trie (xt#xts)\<close> paths.simps 
+      using \<open>(x # (xs' @ xs'')) \<in> set (paths (MP_Trie (xt # xts)))\<close>
+      unfolding \<open>t = MP_Trie (xt#xts)\<close> paths.simps 
       by force
 
     have "distinct (map fst (xt#xts))"
-      using Cons.prems(1) unfolding \<open>t = IO_Trie (xt#xts)\<close> by simp
+      using Cons.prems(1) unfolding \<open>t = MP_Trie (xt#xts)\<close> by simp
     then have "t'' = t'"
       using \<open>(x,t') \<in> set (xt#xts)\<close> \<open>(x,t'') \<in> set (xt#xts)\<close>
       by (meson eq_key_imp_eq_value)  
     then have "xs'@xs'' \<in> set (paths t')"
       using \<open>(xs' @ xs'') \<in> set (paths t'')\<close> by auto
     then show "False"
-      using \<open>xs'' \<noteq> []\<close> Cons.IH[OF \<open>io_trie_invar t'\<close> \<open>xs' \<in> set (paths t')\<close>] by blast
+      using \<open>xs'' \<noteq> []\<close> Cons.IH[OF \<open>mp_trie_invar t'\<close> \<open>xs' \<in> set (paths t')\<close>] by blast
   qed
 qed
             
@@ -338,7 +334,7 @@ qed
 lemma paths_order :
   assumes "set ts = set ts'"
   and     "length ts = length ts'" (* length requirement not actually necessary *)
-shows "set (paths (IO_Trie ts)) = set (paths (IO_Trie ts'))"
+shows "set (paths (MP_Trie ts)) = set (paths (MP_Trie ts'))"
   using assms(2,1) proof (induction ts ts' rule: list_induct2)
   case Nil
   then show ?case by auto
@@ -386,7 +382,7 @@ qed
 
 
 lemma paths_insert_maximal :
-  assumes "io_trie_invar t" 
+  assumes "mp_trie_invar t" 
   shows "set (paths (insert xs t)) = (if (\<exists> xs' . xs@xs' \<in> set (paths t))
                                          then set (paths t)
                                          else Set.insert xs (set (paths t) - {xs' . \<exists> xs'' . xs'@xs'' = xs}))" 
@@ -405,16 +401,16 @@ next
   next
     case False
     
-    then obtain xt xts where "t = IO_Trie (xt#xts)"
-      by (metis IO_Tree.empty_def height.cases)
-    then have "t = IO_Trie ((fst xt, snd xt)#xts)" 
+    then obtain xt xts where "t = MP_Trie (xt#xts)"
+      by (metis empty_def height.cases)
+    then have "t = MP_Trie ((fst xt, snd xt)#xts)" 
       by auto
 
     have "distinct (map fst (xt#xts))"
-      using Cons.prems \<open>t = IO_Trie (xt#xts)\<close> by auto
+      using Cons.prems \<open>t = MP_Trie (xt#xts)\<close> by auto
 
      have "(paths t) = concat (map (\<lambda>(x, t). map ((#) x) (paths t)) (xt # xts))"
-      unfolding \<open>t = IO_Trie ((fst xt, snd xt)#xts)\<close> by simp
+      unfolding \<open>t = MP_Trie ((fst xt, snd xt)#xts)\<close> by simp
     then have "set (paths t) = {x#xs | x xs t . (x,t) \<in> set (xt#xts) \<and> xs \<in> set (paths t)}"
       by auto
     then have "Set.insert (x#xs) (set (paths t)) = Set.insert (x#xs) {x#xs | x xs t . (x,t) \<in> set (xt#xts) \<and> xs \<in> set (paths t)}"
@@ -427,35 +423,35 @@ next
         by (metis in_set_conv_nth list_map_source_elem)
       then have "((xt#xts) ! i) = (x,snd ((xt#xts) ! i))" by auto
 
-      have "io_trie_invar (snd ((xt # xts) ! i))"
-        using Cons.prems \<open>i < length (xt#xts)\<close> unfolding \<open>t = IO_Trie (xt#xts)\<close>
-        by (metis \<open>(xt # xts) ! i = (x, snd ((xt # xts) ! i))\<close> in_set_zipE io_trie_invar.simps nth_mem zip_map_fst_snd) 
+      have "mp_trie_invar (snd ((xt # xts) ! i))"
+        using Cons.prems \<open>i < length (xt#xts)\<close> unfolding \<open>t = MP_Trie (xt#xts)\<close>
+        by (metis \<open>(xt # xts) ! i = (x, snd ((xt # xts) ! i))\<close> in_set_zipE mp_trie_invar.simps nth_mem zip_map_fst_snd) 
 
 
-      have "insert (x#xs) t = IO_Trie (take i (xt # xts) @ [(x, IO_Tree.insert xs (snd ((xt # xts) ! i)))] @ drop (Suc i) (xt # xts))"
-        unfolding \<open>t = IO_Trie (xt#xts)\<close> insert.simps
+      have "insert (x#xs) t = MP_Trie (take i (xt # xts) @ [(x, insert xs (snd ((xt # xts) ! i)))] @ drop (Suc i) (xt # xts))"
+        unfolding \<open>t = MP_Trie (xt#xts)\<close> insert.simps
         unfolding update_assoc_list_with_default_key_found[OF \<open>distinct (map fst (xt#xts))\<close> \<open>i < length (xt#xts)\<close> \<open>fst ((xt#xts) ! i) = x\<close>]
         by simp
       
-      then have "set (paths (insert (x#xs) t)) = set (paths (IO_Trie (take i (xt # xts) @ [(x, IO_Tree.insert xs (snd ((xt # xts) ! i)))] @ drop (Suc i) (xt # xts))))"
+      then have "set (paths (insert (x#xs) t)) = set (paths (MP_Trie (take i (xt # xts) @ [(x, insert xs (snd ((xt # xts) ! i)))] @ drop (Suc i) (xt # xts))))"
         by simp
-      also have "... = set (paths (IO_Trie ((x, IO_Tree.insert xs (snd ((xt # xts) ! i))) # (take i (xt # xts) @ drop (Suc i) (xt # xts)))))"
-        using paths_order[of "(take i (xt # xts) @ [(x, IO_Tree.insert xs (snd ((xt # xts) ! i)))] @ drop (Suc i) (xt # xts))" "((x, IO_Tree.insert xs (snd ((xt # xts) ! i))) # (take i (xt # xts) @ drop (Suc i) (xt # xts)))"]
+      also have "... = set (paths (MP_Trie ((x, insert xs (snd ((xt # xts) ! i))) # (take i (xt # xts) @ drop (Suc i) (xt # xts)))))"
+        using paths_order[of "(take i (xt # xts) @ [(x, insert xs (snd ((xt # xts) ! i)))] @ drop (Suc i) (xt # xts))" "((x, insert xs (snd ((xt # xts) ! i))) # (take i (xt # xts) @ drop (Suc i) (xt # xts)))"]
         by force
-      also have "... = set ((map ((#) x) (paths (IO_Tree.insert xs (snd ((xt # xts) ! i))))) @ (concat (map (\<lambda>(x, t). map ((#) x) (paths t)) (take i (xt # xts) @ drop (Suc i) (xt # xts)))))"
+      also have "... = set ((map ((#) x) (paths (insert xs (snd ((xt # xts) ! i))))) @ (concat (map (\<lambda>(x, t). map ((#) x) (paths t)) (take i (xt # xts) @ drop (Suc i) (xt # xts)))))"
         unfolding paths.simps by force
       finally have "set (paths (insert (x#xs) t)) = 
-                      set (map ((#) x) (paths (IO_Tree.insert xs (snd ((xt # xts) ! i))))) 
+                      set (map ((#) x) (paths (insert xs (snd ((xt # xts) ! i))))) 
                       \<union> set (concat (map (\<lambda>(x, t). map ((#) x) (paths t)) (take i (xt # xts) @ drop (Suc i) (xt # xts))))"
         by force
-      also have "\<dots> = (image ((#) x) (set (paths (IO_Tree.insert xs (snd ((xt # xts) ! i))))))
+      also have "\<dots> = (image ((#) x) (set (paths (insert xs (snd ((xt # xts) ! i))))))
                       \<union> set (concat (map (\<lambda>(x, t). map ((#) x) (paths t)) (take i (xt # xts) @ drop (Suc i) (xt # xts))))"
         by auto
       finally have pi1: "set (paths (insert (x#xs) t)) = 
                       image ((#) x) (if \<exists>xs'. xs @ xs' \<in> set (paths (snd ((xt # xts) ! i))) then set (paths (snd ((xt # xts) ! i)))
                                                                                            else Set.insert xs (set (paths (snd ((xt # xts) ! i))) - {xs'. \<exists>xs''. xs' @ xs'' = xs}))
                        \<union> set (concat (map (\<lambda>(x, t). map ((#) x) (paths t)) (take i (xt # xts) @ drop (Suc i) (xt # xts))))"
-        unfolding Cons.IH[OF \<open>io_trie_invar (snd ((xt # xts) ! i))\<close>] by blast
+        unfolding Cons.IH[OF \<open>mp_trie_invar (snd ((xt # xts) ! i))\<close>] by blast
 
 
 
@@ -466,8 +462,8 @@ next
         using \<open>i < length (xt#xts)\<close> by auto
 
 
-      have "set (paths t) = set (paths (IO_Trie ((x,snd ((xt#xts) ! i)) # ((take i (xt # xts) @ drop (Suc i) (xt # xts))))))"
-        unfolding \<open>t = IO_Trie (xt#xts)\<close> 
+      have "set (paths t) = set (paths (MP_Trie ((x,snd ((xt#xts) ! i)) # ((take i (xt # xts) @ drop (Suc i) (xt # xts))))))"
+        unfolding \<open>t = MP_Trie (xt#xts)\<close> 
         using paths_order[OF po1 po2] by assumption
       also have "\<dots> = set ((map ((#) x) (paths (snd ((xt # xts) ! i)))) @ (concat (map (\<lambda>(x, t). map ((#) x) (paths t)) (take i (xt # xts) @ drop (Suc i) (xt # xts)))))"
         unfolding paths.simps by auto
@@ -487,7 +483,7 @@ next
                                                          \<union> set (concat (map (\<lambda>(x, t). map ((#) x) (paths t)) (take i (xt # xts) @ drop (Suc i) (xt # xts))))"
           using pi1 by auto
 
-        have "set (paths (IO_Tree.insert (x # xs) t)) = set (paths t)"
+        have "set (paths (insert (x # xs) t)) = set (paths t)"
           unfolding pi1' pi2 by simp
         moreover have "\<exists>xs'. (x # xs) @ xs' \<in> set (paths t)"
           using True unfolding pi2 by force
@@ -588,24 +584,24 @@ next
           using x2 by blast
           
 
-        have "set (paths (IO_Tree.insert (x # xs) t)) = Set.insert (x # xs) (set (paths t) - {xs'. \<exists>xs''. xs' @ xs'' = x # xs})"
+        have "set (paths (insert (x # xs) t)) = Set.insert (x # xs) (set (paths t) - {xs'. \<exists>xs''. xs' @ xs'' = x # xs})"
           unfolding pi1' pi2 x1 * by blast
         then show ?thesis
           using x3 by simp 
       qed
     next
       case False
-      have "insert (x#xs) t = IO_Trie (xt # (xts @ [(x, IO_Tree.insert xs empty)]))"
-        unfolding \<open>t = IO_Trie (xt#xts)\<close> insert.simps
+      have "insert (x#xs) t = MP_Trie (xt # (xts @ [(x, insert xs empty)]))"
+        unfolding \<open>t = MP_Trie (xt#xts)\<close> insert.simps
         unfolding update_assoc_list_with_default_key_not_found[OF \<open>distinct (map fst (xt#xts))\<close> False]
         by simp
       
-      have "(paths (IO_Trie (xt # (xts @ [(x, IO_Tree.insert xs empty)])))) = concat (map (\<lambda>(x, t). map ((#) x) (paths t)) (xt # xts @ [(x, IO_Tree.insert xs empty)]))"
+      have "(paths (MP_Trie (xt # (xts @ [(x, insert xs empty)])))) = concat (map (\<lambda>(x, t). map ((#) x) (paths t)) (xt # xts @ [(x, insert xs empty)]))"
         unfolding paths.simps empty_def by simp
       also have "... = (concat (map (\<lambda>(x, t). map ((#) x) (paths t)) (xt # xts))) @ (map ((#) x) (paths (insert xs empty))) "
         by auto
       finally have "paths (insert (x#xs) t) = (paths t) @ [x#xs]"
-        unfolding \<open>insert (x#xs) t = IO_Trie (xt # (xts @ [(x, IO_Tree.insert xs empty)]))\<close>
+        unfolding \<open>insert (x#xs) t = MP_Trie (xt # (xts @ [(x, insert xs empty)]))\<close>
                   \<open>(paths t) = concat (map (\<lambda>(x, t). map ((#) x) (paths t)) (xt # xts))\<close>[symmetric]
                   paths_insert_empty 
         by auto
@@ -631,12 +627,12 @@ qed
 
 
 
-fun insert_all :: "'a list list \<Rightarrow> 'a io_trie" where
+fun insert_all :: "'a list list \<Rightarrow> 'a mp_trie" where
   "insert_all seqs = foldr insert seqs empty"
 
  
 
-lemma insert_all_invar : "io_trie_invar (insert_all xs)"
+lemma insert_all_invar : "mp_trie_invar (insert_all xs)"
   using empty_invar insert_invar by (induction xs; auto)
 
 lemma insert_all_paths :
@@ -656,28 +652,28 @@ next
   have "insert_all (x#x'#xs) = insert x (insert x' (insert_all xs))" by auto
   have "insert_all (x#x'#xs) = insert x (insert_all (x'#xs))" by auto
 
-  have "io_trie_invar (insert x' (insert_all xs))"
+  have "mp_trie_invar (insert x' (insert_all xs))"
     using insert_all_invar insert_invar by metis
   have "(insert x' (insert_all xs)) = insert_all (x'#xs)" by auto
 
 
-  thm paths_insert_maximal[OF \<open>io_trie_invar (insert x' (insert_all xs))\<close>, of x]
+  thm paths_insert_maximal[OF \<open>mp_trie_invar (insert x' (insert_all xs))\<close>, of x]
 
-  show ?case proof (cases "\<exists>xs'. x @ xs' \<in> set (paths (IO_Tree.insert x' (insert_all xs)))")
+  show ?case proof (cases "\<exists>xs'. x @ xs' \<in> set (paths (insert x' (insert_all xs)))")
     case True
-    then have "set (paths (IO_Tree.insert x (IO_Tree.insert x' (insert_all xs)))) = set (paths (IO_Tree.insert x' (insert_all xs)))"
-      using paths_insert_maximal[OF \<open>io_trie_invar (insert x' (insert_all xs))\<close>, of x] by simp
-    then have "set (paths (IO_Tree.insert x (insert_all (x' # xs)))) = set (paths (insert_all (x' # xs)))"
+    then have "set (paths (insert x (insert x' (insert_all xs)))) = set (paths (insert x' (insert_all xs)))"
+      using paths_insert_maximal[OF \<open>mp_trie_invar (insert x' (insert_all xs))\<close>, of x] by simp
+    then have "set (paths (insert x (insert_all (x' # xs)))) = set (paths (insert_all (x' # xs)))"
       unfolding \<open>(insert x' (insert_all xs)) = insert_all (x'#xs)\<close> 
       by assumption
     then have "set (paths (insert_all (x#x'#xs))) = {y \<in> set (x' # xs). \<nexists>y'. y' \<noteq> [] \<and> y @ y' \<in> set (x' # xs)}"
       unfolding Cons \<open>insert_all (x#x'#xs) = insert x (insert_all (x'#xs))\<close>
       by assumption
 
-    show ?thesis proof (cases "x \<in> set (paths (IO_Tree.insert x' (insert_all xs)))")
+    show ?thesis proof (cases "x \<in> set (paths (insert x' (insert_all xs)))")
       case True
       then have "x \<in> set (x'#xs)"
-        using \<open>set (paths (IO_Tree.insert x (IO_Tree.insert x' (insert_all xs)))) = set (paths (IO_Tree.insert x' (insert_all xs)))\<close> \<open>set (paths (insert_all (x # x' # xs))) = {y \<in> set (x' # xs). \<nexists>y'. y' \<noteq> [] \<and> y @ y' \<in> set (x' # xs)}\<close> by auto
+        using \<open>set (paths (insert x (insert x' (insert_all xs)))) = set (paths (insert x' (insert_all xs)))\<close> \<open>set (paths (insert_all (x # x' # xs))) = {y \<in> set (x' # xs). \<nexists>y'. y' \<noteq> [] \<and> y @ y' \<in> set (x' # xs)}\<close> by auto
       then show ?thesis 
         unfolding \<open>set (paths (insert_all (x#x'#xs))) = {y \<in> set (x' # xs). \<nexists>y'. y' \<noteq> [] \<and> y @ y' \<in> set (x' # xs)}\<close> by auto
     next
@@ -687,7 +683,7 @@ next
       proof -
         obtain xs' where "xs' \<noteq> []" and "x @ xs' \<in>  {y \<in> set (x' # xs). \<nexists>y'. y' \<noteq> [] \<and> y @ y' \<in> set (x' # xs)}"
           using True False
-          by (metis \<open>insert_all (x # x' # xs) = IO_Tree.insert x (IO_Tree.insert x' (insert_all xs))\<close> \<open>set (paths (IO_Tree.insert x (IO_Tree.insert x' (insert_all xs)))) = set (paths (IO_Tree.insert x' (insert_all xs)))\<close> \<open>set (paths (insert_all (x # x' # xs))) = {y \<in> set (x' # xs). \<nexists>y'. y' \<noteq> [] \<and> y @ y' \<in> set (x' # xs)}\<close> append_Nil2) 
+          by (metis \<open>insert_all (x # x' # xs) = insert x (insert x' (insert_all xs))\<close> \<open>set (paths (insert x (insert x' (insert_all xs)))) = set (paths (insert x' (insert_all xs)))\<close> \<open>set (paths (insert_all (x # x' # xs))) = {y \<in> set (x' # xs). \<nexists>y'. y' \<noteq> [] \<and> y @ y' \<in> set (x' # xs)}\<close> append_Nil2) 
         then have s1: "{y \<in> set (x # x' # xs). \<nexists>y'. y' \<noteq> [] \<and> y @ y' \<in> set (x # x' # xs)} = {y \<in> set (x' # xs). \<nexists>y'. y' \<noteq> [] \<and> y @ y' \<in> set (x # x' # xs)}"
           by auto 
             
@@ -720,9 +716,9 @@ next
     case False
     
 
-    then have *: "set (paths (IO_Tree.insert x (IO_Tree.insert x' (insert_all xs)))) 
-                = Set.insert x (set (paths (IO_Tree.insert x' (insert_all xs))) - {xs'. \<exists>xs''. xs' @ xs'' = x})"
-      using paths_insert_maximal[OF \<open>io_trie_invar (insert x' (insert_all xs))\<close>, of x] by simp
+    then have *: "set (paths (insert x (insert x' (insert_all xs)))) 
+                = Set.insert x (set (paths (insert x' (insert_all xs))) - {xs'. \<exists>xs''. xs' @ xs'' = x})"
+      using paths_insert_maximal[OF \<open>mp_trie_invar (insert x' (insert_all xs))\<close>, of x] by simp
 
     have f: "\<nexists>xs'. x @ xs' \<in> {y \<in> set (x' # xs). \<nexists>y'. y' \<noteq> [] \<and> y @ y' \<in> set (x' # xs)}"
       using False
@@ -866,6 +862,7 @@ qed
 value "pow_list (upto 1 10)"
 value "insert_all (pow_list (upto 1 10))"
 value "paths (insert_all (pow_list (upto 1 10)))"
+
 
 
 end 
